Make batch sampling example a function [foxtrot]

theories/foxtrot/examples/batch_sampling_seq.v
@@ -3,31 +3,34 @@ From clutch.foxtrot Require Import foxtrot par spawn batch_sampling.
 (** * Sequential version of the batch sampler*)
 Section batch.
   Variable N M:nat.
-  Definition seq_batch_prog : expr :=
+  Definition seq_batch_prog : val :=
+    λ: "_",
     let: "x" := (rand #N)  in
     let: "y" := (rand #M) in 
     "x" * (#(M+1)) + "y".
 
-  Definition seq_batch_prog' : expr :=
+  Definition seq_batch_prog' : val :=
+    λ: "_",
     let: "α" := alloc #N in
     let: "α'" := alloc #M in
     let: "x" := (rand("α") #N)  in
     let: "y" := (rand("α'") #M) in 
     "x" * (#(M+1)) + "y".
   
-  Definition rand_prog : expr := rand #((S N) * (S M)-1).
+  Definition rand_prog : val := λ: "_", rand #((S N) * (S M)-1).
   
   Section proof.
     Context `{!foxtrotRGS Σ}.
     
     Lemma wp_seq_batch_prog_seq_batch_prog' K j:
-    {{{ j ⤇ fill K seq_batch_prog' }}}
-      seq_batch_prog
+    {{{ j ⤇ fill K (seq_batch_prog' #()) }}}
+      seq_batch_prog #()
       {{{ v, RET v; ∃ v' : val, j ⤇ fill K v' ∗ lrel_nat v v' }}}.
     Proof.
       iIntros (Φ) "Hspec HΦ".
       rewrite /seq_batch_prog'/seq_batch_prog.
       wp_pures.
+      tp_pures j.
       tp_allocnattape j α as "Hα".
       tp_pures j.
       tp_allocnattape j α' as "Hα'".
@@ -51,8 +54,8 @@ Section batch.
     Qed.
     
     Lemma wp_seq_batch_prog'_rand_prog K j:
-    {{{ j ⤇ fill K rand_prog }}}
-      seq_batch_prog'
+    {{{ j ⤇ fill K (rand_prog #()) }}}
+      seq_batch_prog' #()
       {{{ v, RET v; ∃ v' : val, j ⤇ fill K v' ∗ lrel_nat v v' }}}.
     Proof.
       iIntros (Φ) "Hspec HΦ".
@@ -62,6 +65,7 @@ Section batch.
       wp_pures.
       wp_alloctape α' as "Hα'".
       wp_pures.
+      tp_pures j.
       iMod (pupd_couple_two_tapes_rand _ _ (coupling_f M) with "[$Hα][$][$]") as "(%n&%m&Hα&Hα'&Hspec &%&%)".
       - rewrite TCEq_eq. by erewrite Nat2Z.id.
       - rewrite TCEq_eq. by erewrite Nat2Z.id.
@@ -87,8 +91,8 @@ Section batch.
     Context `{!foxtrotRGS Σ, Hspawn: !spawnG Σ}.
 
     Lemma wp_batch_prog'_seq_batch_prog K j:
-    {{{ j ⤇ fill K seq_batch_prog }}}
-      batch_prog' N M
+    {{{ j ⤇ fill K (seq_batch_prog #()) }}}
+      batch_prog' N M #()
       {{{ v, RET v; ∃ v' : val, j ⤇ fill K v' ∗ lrel_nat v v' }}}.
     Proof using Hspawn.
       iIntros (Φ) "Hspec HΦ".
@@ -98,6 +102,7 @@ Section batch.
       wp_pures.
       wp_alloctape α' as "Hα'".
       wp_pures.
+      tp_pures j.
       tp_bind j (rand _)%E.
       iMod (pupd_couple_tape_rand with "[$Hα][$]") as "(%n&Hα&Hspec&%)"; first naive_solver.
       simpl.
@@ -120,41 +125,73 @@ Section batch.
   End proof'.
 
   Lemma seq_batch_prog_refines_rand_prog :
-    ∅ ⊨ seq_batch_prog ≤ctx≤ rand_prog : TNat.
+    ∅ ⊨ seq_batch_prog ≤ctx≤ rand_prog : (TUnit → TNat).
   Proof.
     eapply ctx_refines_transitive with seq_batch_prog';
       apply (refines_sound (#[foxtrotRΣ])); rewrite /interp/=.
     - iIntros. unfold_rel.
       iIntros (K j) "Hspec".
+      wp_pures.
+      iFrame.
+      iModIntro.
+      iIntros (??[->->]).
+      unfold_rel.
+      iModIntro.
+      clear K j.
+      iIntros (K j) "Hspec". 
       wp_apply (wp_seq_batch_prog_seq_batch_prog' with "[$]").
       iIntros (v) "(%&?&?)". iFrame. 
     - iIntros. unfold_rel.
       iIntros (K j) "Hspec".
+      wp_pures.
+      iFrame.
+      iModIntro.
+      iIntros (??[->->]).
+      unfold_rel.
+      iModIntro.
+      clear K j.
+      iIntros (K j) "Hspec". 
       wp_apply (wp_seq_batch_prog'_rand_prog with "[$]").
       iIntros (v) "(%&?&?)". iFrame.
   Qed. 
 
   Lemma rand_prog_refines_seq_batch_prog :
-    ∅ ⊨ rand_prog ≤ctx≤ seq_batch_prog : TNat.
+    ∅ ⊨ rand_prog ≤ctx≤ seq_batch_prog : (TUnit →TNat).
   Proof.
     eapply ctx_refines_transitive with (batch_prog N M); first apply rand_prog_refines_batch_prog.
     eapply ctx_refines_transitive with (batch_prog' N M).
     - apply (refines_sound (#[spawnΣ; foxtrotRΣ])).
       iIntros.
       unfold_rel.
-      iIntros. 
+      iIntros (K j) "Hspec".
+      wp_pures.
+      iFrame.
+      iModIntro.
+      iIntros (??[->->]).
+      unfold_rel.
+      iModIntro.
+      clear K j.
+      iIntros (K j) "Hspec".
       iApply (wp_batch_prog_batch_prog' with "[$]").
       iNext.
       by iIntros.
     - apply (refines_sound (#[spawnΣ; foxtrotRΣ])).
       iIntros. unfold_rel.
-      iIntros.
+      iIntros (K j) "Hspec".
+      wp_pures.
+      iFrame.
+      iModIntro.
+      iIntros (??[->->]).
+      unfold_rel.
+      iModIntro.
+      clear K j.
+      iIntros (K j) "Hspec". 
       wp_apply (wp_batch_prog'_seq_batch_prog with "[$]").
       by iIntros.
   Qed. 
 
   Lemma seq_batch_prog_eq_rand_prog :
-    ∅ ⊨ seq_batch_prog =ctx= rand_prog : TNat.
+    ∅ ⊨ seq_batch_prog =ctx= rand_prog : (TUnit → TNat).
   Proof.
     split; [apply seq_batch_prog_refines_rand_prog|apply rand_prog_refines_seq_batch_prog].
   Qed. 
